# Canonical Order of Operations Index Laws

**By Andrew Lehti**

---

## The Misconceptions of the Standard Order and the Introduction of the Canonical Order  

### **The First Misconception**  

A negative times a negative equals a positive. While technically true, it is actually a negative cancels a negative and there must be two negatives already present. This concept is often misapplied. The root cause lies in efforts to simplify exponentials by framing them as repeated multiplication, such as:

$$
x^n = x \times x \times \ldots \text{ (n times)}
$$

While again technically accurate, many stop there, and this explanation fosters a conflation of multiplication and exponentiation, leading to misunderstandings about the exponential operator.

---

### **The Second Misconception**  

Operators act independently of other operators. Many misunderstand the role of the negative sign in expressions like $-5^2$, incorrectly treating the negative as part of the base or assuming it interacts with the exponent. This confusion also extends to roots, where $\sqrt{x}$ is underemphasized as a fractional exponent.

A deeper logical fallacy arises when attempting to extend negative bases into fractional exponents. For example:  

$$
(-5)^5 = -3125\ and\ (-5)^6 = 15625
$$

But what would $(-5)^{5.5}$ equal? This is where some got confused and where arithmetic begins breaking into an **imaginary realm** of understanding, as fractional exponents involving negatives inherently introduce imaginary numbers:

$$
(-5)^{5.5} = \sqrt{-3125^5}
$$

This represents a breakdown in practical arithmetic and shifts into theoretical constructs like complex numbers, which are often presented as if they are "real" when their interpretation is not intuitive or tied to the physical world.

---

### **The Third Misconception**  

The expression $-5^2 = -25$ confuses many due to failings in the education system. The Standard Order of Operations resolves this as:

$$
(-5)^2 = 25
$$

This is interpreted as $(-5)(-5) = 25$. However, this conflates multiplication and exponentiation, leading to ambiguity that the Canonical framework eliminates.

---

### **The Fourth Misconception**  

The Order of Operations requires that parentheses must always be resolved first, yet the Standard Order breaks this requirement, which is misleading. For example, in $(-5)^2$:

- Parentheses group the base, $-5$, for the exponentiation operation.  
- The combination of multiplication $((-5)(-5))$ with exponentiation is often how $(-5)^2$ is misinterpreted.  

Exponentiation inherently acts on the base, independent of surrounding operators, as it affects only the leftmost number. Correct resolution ensures only one base is acted upon, provided the base does not contain variables.

---

### **The Fifth Misconception**  

Negative signs are unaffected by other operators. For example:

$$
-5 \times 6 = -30\ not\ 30
$$

Similarly:

$$
(-5) \times 6 = -30\ not\ 30
$$

---

### **The Sixth Misconception**  

If a result cannot be inverted like its incremental counterparts, it is inherently flawed. For instance:

- $+1, +2, +3$ can be undone with $-1, -2, -3$, ensuring mathematical consistency.  

However, consider:

$$(-2)^2 = 4$$
$$(-2)^3 = -8$$
$$(-2)^4 = 16$$

These results cannot be consistently undone using operations such as $\sqrt{4}$, $\sqrt[3]{-8}$, or $\sqrt[4]{16}$, revealing flaws in the Standard Order.

---

## The Canonical Order  

The **Canonical Order** eliminates ambiguities caused by symbols like the square root, which introduces errors across mathematical literature due to inconsistent sign placement interpretations. For example:

$$
-\sqrt{-5}\ simplifies\ to\ -(-5^{1/2})
$$

Such ambiguities create deeper errors as complexity increases.

**The Canonical Order prioritizes understanding over aesthetics.**

---

## Clarifications under the Canonical Order  

$$
x^{\frac{2}{3}} = the\ **cube\ root\ of\ x^2$**\ or\ \sqrt[3]{x^2}
$$

$$
x^{\frac{3}{4}} = the\ **fourth\ root\ of\ x^3$**\ or\ \sqrt[4]{x^3}
$$

---

## Identifying Biases in the Standard Order  

### **The First Bias**  

In the Standard Order, we treat $(-5)^2$ as:

$$
(-5)^2 = (-5)(-5) = 25
$$

However, we do not treat $(-5) \times 2$ in the same way, instead solving as:

$$
(-5) \times 2 = 0 - (5 \times 2) = -10
$$

---

### **The Second Bias**  

In the Standard Order:

$$
(5^2)^4 = 5^{2 \times 4} = 5^8 = 390625
$$

But introducing a negative base creates inconsistent logic:

$$
(-5^2)^4 = (-25)^4 = (-25)(-25)(-25)(-25) = 390625
$$

Under the Canonical Order, such inconsistencies are discarded. Instead, operations are performed consistently and logically:

$$
(-5^2)^4 = -5^{2 \times 4} = -5^8 = -390625
$$

$$
(-5)^4 = (-5^1)^4 = -5^{1 \times 4} = -625
$$

---

### Rewriting Roots as Powers (Canonical Order)

#### **Single Roots**
- $\sqrt{a} = a^{\frac{1}{2}}$
- $\sqrt[3]{a} = a^{\frac{1}{3}}$
- $\sqrt[4]{a} = a^{\frac{1}{4}}$
- $\sqrt[n]{a} = a^{\frac{1}{n}}$

#### **Roots with Exponents**
- $\sqrt{a^m} = a^{\frac{m}{2}}$
- $\sqrt[3]{a^m} = a^{\frac{m}{3}}$
- $\sqrt[4]{a^m} = a^{\frac{m}{4}}$
- $\sqrt[n]{a^m} = a^{\frac{m}{n}}$

#### **Parentheses and Power Distribution**
- $(\sqrt{a})^m = (a^{\frac{1}{2}})^m = a^{\frac{m}{2}}$
- $(\sqrt[3]{a})^m = (a^{\frac{1}{3}})^m = a^{\frac{m}{3}}$
- $(\sqrt[n]{a})^m = (a^{\frac{1}{n}})^m = a^{\frac{m}{n}}$

#### **Nested Roots**
- $\sqrt{\sqrt{a}} = \sqrt[4]{a} = a^{\frac{1}{4}}$
- $\sqrt{\sqrt[3]{a}} = \sqrt[6]{a} = a^{\frac{1}{6}}$
- $\sqrt[3]{\sqrt{a}} = \sqrt[6]{a} = a^{\frac{1}{6}}$
- $\sqrt[3]{\sqrt[3]{a}} = \sqrt[9]{a} = a^{\frac{1}{9}}$

#### **Negative Roots**
- $-\sqrt{a} = -a^{\frac{1}{2}}$
- $-\sqrt[3]{a} = -a^{\frac{1}{3}}$
- $-\sqrt[n]{a^m} = -a^{\frac{m}{n}}$

#### **Reciprocal Roots**
- $\frac{1}{\sqrt{a}} = a^{-\frac{1}{2}}$
- $\frac{1}{\sqrt[3]{a}} = a^{-\frac{1}{3}}$
- $\frac{1}{\sqrt[n]{a}} = a^{-\frac{1}{n}}$
- $\frac{1}{\sqrt[n]{a^m}} = a^{-\frac{m}{n}}$

#### **Negative Reciprocal Roots**
- $-\frac{1}{\sqrt{a}} = -a^{-\frac{1}{2}}$
- $-\frac{1}{\sqrt[3]{a}} = -a^{-\frac{1}{3}}$
- $-\frac{1}{\sqrt[n]{a}} = -a^{-\frac{1}{n}}$

#### **Combined Power and Root**
- $\sqrt[n]{a^m} = a^{\frac{m}{n}}$
- $(\sqrt[n]{a})^m = (a^{\frac{1}{n}})^m = a^{\frac{m}{n}}$
---

### I. **Implicit Power of 1 for Any Number or Variable**
$a = a^1$

Every number or variable is always implicitly raised to the power of 1, even if not explicitly written. This foundational rule enables consistent application of exponent laws, establishing each base as $a^1$.

---

### II. **Multiplying Powers with the Same Base**
$a^m \times a^n = a^{m+n}$

When multiplying expressions with the same base, add the exponents. This rule consolidates powers correctly: $a^2 \times a^3 = a^{2+3} = a^5$.

---

### III. **Dividing Powers with the Same Base**
$\frac{a^m}{a^n} = a^{m-n} \quad \text{(where } a \neq 0)$

When dividing expressions with the same base, subtract the exponent of the denominator from that of the numerator. This ensures accurate reduction: $\frac{a^5}{a^2} = a^{5-2} = a^3$.

---

### IV. **Power of a Power**
$(a^m)^n = a^{m \times n} = a^{mn}$

When an exponentiated expression is raised to another power, multiply the exponents. Following the order of operations, parentheses must be removed first, achieved here by applying this rule: $(a^2)^3 = a^{2 \times 3} = a^6$.

---

### V. **Parenthesized Base Raised to a Power**
$(a)^m = (a^1)^m = a^{1 \times m} = a^m$

For a variable or number in parentheses, recognize the base as implicitly raised to the power of 1. According to standard arithmetic rules, each number or variable is treated as $a^1$, which enables removal of parentheses and application of the power: $(a)^m = (a^1)^m = a^{1 \times m} = a^m$.

---

### VI. **Zero Exponent Law**
$a^0 = 1 \quad \text{(where } a \neq 0)$

Any non-zero number raised to the power of zero is always equal to 1. This universal law applies to all bases: $5^0 = 1$.

---

### VII. **Negative Exponent Law**
$a^{-m} = \frac{1}{a^m} \quad \text{(where } a \neq 0)$

A negative exponent inverts the base, resulting in the reciprocal of the base raised to the positive exponent: $a^{-2} = \frac{1}{a^2}$.

---

### VIII. **Distributing a Power over Multiplication**
$(ab)^m = a^m \times b^m$

When a product is raised to a power, distribute the exponent to each factor within the parentheses. This step is necessary for accurate results: $(2x)^3 = 2^3 \times x^3 = 8x^3$.

---

### IX. **Distributing a Power over Division**
$\left(\frac{a}{b}\right)^m = \frac{a^m}{b^m} \quad \text{(where } b \neq 0)$

When a fraction is raised to a power, distribute the exponent to both numerator and denominator. This ensures proper handling of fractional powers: $\left(\frac{2}{3}\right)^2 = \frac{2^2}{3^2} = \frac{4}{9}$.

---

### X. **Power as the Inverse (Root Interpretation)**
$a^{\frac{1}{n}} = \sqrt[n]{a}$

Raising a number to the power of $\frac{1}{n}$ equates to taking the nth root of that number: $a^{\frac{1}{2}} = \sqrt{a}$.

---

### XI. **Fractional Exponents Representing Power and Root**
$a^{\frac{m}{n}} = \sqrt[n]{a^m}$
A fractional exponent implies both a power and a root, with the denominator as the root and the numerator as the power. This interpretation is essential: $a^{\frac{3}{2}} = \sqrt{a^3}$.

---

### XII. **Power of 1**
$a^1 = a$

Any number raised to the power of 1 remains unchanged. This rule is absolute: $7^1 = 7$.

---

### XIII. **Zero to a Positive Exponent**
$0^m = 0 \quad \text{(for } m > 0)$

Zero raised to any positive exponent is always zero, without exception: $0^5 = 0$.

---

### XIV. **Interpreting Negative Signs with Powers**
For expressions with negative bases raised to powers, the negative sign remains external when the base is implicitly raised to the power of 1. Applying the implicit unity concept allows consistent handling of negatives:

$(-a)^m = (-a^1)^m = -a^{1 \times m} = -a^m$

This interpretation maintains the negative outside the exponentiated term, ensuring proper evaluation.

---

### **The Law of Implicit Unity in Exponential Powers**
This law establishes that every base, whether explicitly stated or in parentheses, is implicitly raised to the power of 1, enabling the removal of parentheses without altering the expression. It reinforces that parentheses containing bases should be viewed as $a^1$, ensuring consistent exponentiation:

1. For any term in parentheses, the base can be considered raised to the implicit power of 1.
   
   $(a)^m = (a^1)^m = a^{1 \times m} = a^m$

2. In cases involving negatives, such as $(-a)^m$, apply this implicit unity to the absolute base:
   
   $(-a)^m = (-a^1)^m = -a^{1 \times m} = -a^m$
